Updated examples.

tests/zigbee/headerAdd.cal.bpl
@@ -9,11 +9,15 @@ type CType = <a>[Chan a]int;
 type MType = <a>[Chan a][int]a;
 type Obj = <a>[Field a]a;
 type HType = [Ref]Obj;
+type ModeType = [Actor]int;
 
 var M: MType;
 var C: CType;
 var R: CType;
 var I: CType;
+var B: CType;
+var Mode: ModeType;
+var I#sub: CType;
 
 var H: HType;
 
@@ -54,6 +58,10 @@ function {:bvbuiltin "bvule"} AT#BvUle8(a: bv8, b: bv8): bool;
 function {:bvbuiltin "bvult"} AT#BvUlt8(a: bv8, b: bv8): bool;
 function {:bvbuiltin "bvuge"} AT#BvUge8(a: bv8, b: bv8): bool;
 function {:bvbuiltin "bvugt"} AT#BvUgt8(a: bv8, b: bv8): bool;
+function {:bvbuiltin "bvsle"} AT#BvSle8(a: bv8, b: bv8): bool;
+function {:bvbuiltin "bvslt"} AT#BvSlt8(a: bv8, b: bv8): bool;
+function {:bvbuiltin "bvsge"} AT#BvSge8(a: bv8, b: bv8): bool;
+function {:bvbuiltin "bvsgt"} AT#BvSgt8(a: bv8, b: bv8): bool;
 function AT#BvXor8(a: bv8, b: bv8): bv8;
 
 axiom (forall a,b: bv8 :: AT#BvXor8(a,b) == AT#BvAnd8(AT#BvOr8(a,b), AT#BvNot8(AT#BvAnd8(a,b))) );
@@ -63,7 +71,7 @@ axiom (forall a,b: bv8 :: AT#BvXor8(a,b) == AT#BvAnd8(AT#BvOr8(a,b), AT#BvNot8(A
 // ---------------------------------------------------------------
 
 procedure headerAdd#init#0()
-  modifies C, R, M, I, H;
+  modifies C, R, M, I, H, I#sub;
 {
   var pl_bits: Chan (bv8);
   var data: Chan (bv8);
@@ -75,21 +83,22 @@ procedure headerAdd#init#0()
   var data_out: bv8;
   var St: int;
   assume (pl_bits != data) && (pl_bits != len) && (data != len);
-  assume R[pl_bits] == 0;
-  assume C[data] == 0;
-  assume C[len] == 0;
+  assume HEADER_LEN == 5;
+  assume (I[pl_bits] == 0) && (R[pl_bits] == 0) && (C[pl_bits] == 0);
+  assume (I[data] == 0) && (R[data] == 0) && (C[data] == 0);
+  assume (I[len] == 0) && (R[len] == 0) && (C[len] == 0);
   octet_index := 0bv8;
   octet_count := 14bv8;
   St := 0;
-  assert {:msg "25.12: Initialization might not establish the invariant (#0)"} AT#BvUle8(0bv8, octet_index);
-  assert {:msg "26.12: Initialization might not establish the invariant (#1)"} AT#BvUle8(octet_index, octet_count);
-  assert {:msg "27.12: Initialization might not establish the invariant (#2)"} octet_count == 14bv8;
-  assert {:msg "29.12: Initialization might not establish the invariant (#3)"} (St == 1) ==> AT#BvUle8(octet_index, 5bv8);
-  assert {:msg "30.12: Initialization might not establish the invariant (#4)"} (St == 2) ==> AT#BvUlt8(5bv8, octet_index);
-  assert {:msg "31.12: Initialization might not establish the invariant (#5)"} (0 <= St) && (St <= 2);
+  assert {:msg "headerAdd.cal(25.12): Initialization might not establish the invariant (#0)"} AT#BvUle8(0bv8, octet_index);
+  assert {:msg "headerAdd.cal(26.12): Initialization might not establish the invariant (#1)"} AT#BvUle8(octet_index, octet_count);
+  assert {:msg "headerAdd.cal(27.12): Initialization might not establish the invariant (#2)"} octet_count == 14bv8;
+  assert {:msg "headerAdd.cal(29.12): Initialization might not establish the invariant (#3)"} (St == 1) ==> AT#BvUle8(octet_index, 5bv8);
+  assert {:msg "headerAdd.cal(30.12): Initialization might not establish the invariant (#4)"} (St == 2) ==> AT#BvUlt8(5bv8, octet_index);
+  assert {:msg "headerAdd.cal(31.12): Initialization might not establish the invariant (#5)"} (0 <= St) && (St <= 2);
 }
 procedure headerAdd#get_data_len#1()
-  modifies C, R, M, I, H;
+  modifies C, R, M, I, H, I#sub;
 {
   var pl_bits: Chan (bv8);
   var data: Chan (bv8);
@@ -102,15 +111,17 @@ procedure headerAdd#get_data_len#1()
   var St: int;
   var pl_bits#0: bv8;
   assume (pl_bits != data) && (pl_bits != len) && (data != len);
-  assume 0 <= R[pl_bits];
-  assume 0 <= C[data];
-  assume 0 <= C[len];
+  assume HEADER_LEN == 5;
+  assume (0 <= I[pl_bits]) && (I[pl_bits] <= R[pl_bits]) && (R[pl_bits] <= C[pl_bits]);
+  assume (0 <= I[data]) && (I[data] <= R[data]) && (R[data] <= C[data]);
+  assume (0 <= I[len]) && (I[len] <= R[len]) && (R[len] <= C[len]);
   assume AT#BvUle8(0bv8, octet_index);
   assume AT#BvUle8(octet_index, octet_count);
   assume octet_count == 14bv8;
   assume (St == 1) ==> AT#BvUle8(octet_index, 5bv8);
   assume (St == 2) ==> AT#BvUlt8(5bv8, octet_index);
   assume (0 <= St) && (St <= 2);
+  assume 1 <= (C[pl_bits] - R[pl_bits]);
   pl_bits#0 := M[pl_bits][R[pl_bits]];
   R[pl_bits] := R[pl_bits] + 1;
   assume pl_bits#0 == 8bv8;
@@ -120,15 +131,15 @@ procedure headerAdd#get_data_len#1()
   St := 1;
   M[len][C[len]] := octet_count;
   C[len] := C[len] + 1;
-  assert {:msg "25.12: Action at 46.2 might not preserve invariant (#6)"} AT#BvUle8(0bv8, octet_index);
-  assert {:msg "26.12: Action at 46.2 might not preserve invariant (#7)"} AT#BvUle8(octet_index, octet_count);
-  assert {:msg "27.12: Action at 46.2 might not preserve invariant (#8)"} octet_count == 14bv8;
-  assert {:msg "29.12: Action at 46.2 might not preserve invariant (#9)"} (St == 1) ==> AT#BvUle8(octet_index, 5bv8);
-  assert {:msg "30.12: Action at 46.2 might not preserve invariant (#10)"} (St == 2) ==> AT#BvUlt8(5bv8, octet_index);
-  assert {:msg "31.12: Action at 46.2 might not preserve invariant (#11)"} (0 <= St) && (St <= 2);
+  assert {:msg "headerAdd.cal(25.12): Action 'get_data_len' at headerAdd.cal(46.2) might not preserve the invariant (#6)"} AT#BvUle8(0bv8, octet_index);
+  assert {:msg "headerAdd.cal(26.12): Action 'get_data_len' at headerAdd.cal(46.2) might not preserve the invariant (#7)"} AT#BvUle8(octet_index, octet_count);
+  assert {:msg "headerAdd.cal(27.12): Action 'get_data_len' at headerAdd.cal(46.2) might not preserve the invariant (#8)"} octet_count == 14bv8;
+  assert {:msg "headerAdd.cal(29.12): Action 'get_data_len' at headerAdd.cal(46.2) might not preserve the invariant (#9)"} (St == 1) ==> AT#BvUle8(octet_index, 5bv8);
+  assert {:msg "headerAdd.cal(30.12): Action 'get_data_len' at headerAdd.cal(46.2) might not preserve the invariant (#10)"} (St == 2) ==> AT#BvUlt8(5bv8, octet_index);
+  assert {:msg "headerAdd.cal(31.12): Action 'get_data_len' at headerAdd.cal(46.2) might not preserve the invariant (#11)"} (0 <= St) && (St <= 2);
 }
 procedure headerAdd#send_header#2()
-  modifies C, R, M, I, H;
+  modifies C, R, M, I, H, I#sub;
 {
   var pl_bits: Chan (bv8);
   var data: Chan (bv8);
@@ -141,30 +152,32 @@ procedure headerAdd#send_header#2()
   var St: int;
   var pl_bits#0: bv8;
   assume (pl_bits != data) && (pl_bits != len) && (data != len);
-  assume 0 <= R[pl_bits];
-  assume 0 <= C[data];
-  assume 0 <= C[len];
+  assume HEADER_LEN == 5;
+  assume (0 <= I[pl_bits]) && (I[pl_bits] <= R[pl_bits]) && (R[pl_bits] <= C[pl_bits]);
+  assume (0 <= I[data]) && (I[data] <= R[data]) && (R[data] <= C[data]);
+  assume (0 <= I[len]) && (I[len] <= R[len]) && (R[len] <= C[len]);
   assume AT#BvUle8(0bv8, octet_index);
   assume AT#BvUle8(octet_index, octet_count);
   assume octet_count == 14bv8;
   assume (St == 1) ==> AT#BvUle8(octet_index, 5bv8);
   assume (St == 2) ==> AT#BvUlt8(5bv8, octet_index);
   assume (0 <= St) && (St <= 2);
+  assume true;
   assume AT#BvUlt8(octet_index, 5bv8) && (St == 1);
   data_out := Map#Select(Header, octet_index);
   octet_index := AT#BvAdd8(octet_index, 1bv8);
   St := 1;
   M[data][C[data]] := data_out;
   C[data] := C[data] + 1;
-  assert {:msg "25.12: Action at 57.2 might not preserve invariant (#12)"} AT#BvUle8(0bv8, octet_index);
-  assert {:msg "26.12: Action at 57.2 might not preserve invariant (#13)"} AT#BvUle8(octet_index, octet_count);
-  assert {:msg "27.12: Action at 57.2 might not preserve invariant (#14)"} octet_count == 14bv8;
-  assert {:msg "29.12: Action at 57.2 might not preserve invariant (#15)"} (St == 1) ==> AT#BvUle8(octet_index, 5bv8);
-  assert {:msg "30.12: Action at 57.2 might not preserve invariant (#16)"} (St == 2) ==> AT#BvUlt8(5bv8, octet_index);
-  assert {:msg "31.12: Action at 57.2 might not preserve invariant (#17)"} (0 <= St) && (St <= 2);
+  assert {:msg "headerAdd.cal(25.12): Action 'send_header' at headerAdd.cal(57.2) might not preserve the invariant (#12)"} AT#BvUle8(0bv8, octet_index);
+  assert {:msg "headerAdd.cal(26.12): Action 'send_header' at headerAdd.cal(57.2) might not preserve the invariant (#13)"} AT#BvUle8(octet_index, octet_count);
+  assert {:msg "headerAdd.cal(27.12): Action 'send_header' at headerAdd.cal(57.2) might not preserve the invariant (#14)"} octet_count == 14bv8;
+  assert {:msg "headerAdd.cal(29.12): Action 'send_header' at headerAdd.cal(57.2) might not preserve the invariant (#15)"} (St == 1) ==> AT#BvUle8(octet_index, 5bv8);
+  assert {:msg "headerAdd.cal(30.12): Action 'send_header' at headerAdd.cal(57.2) might not preserve the invariant (#16)"} (St == 2) ==> AT#BvUlt8(5bv8, octet_index);
+  assert {:msg "headerAdd.cal(31.12): Action 'send_header' at headerAdd.cal(57.2) might not preserve the invariant (#17)"} (0 <= St) && (St <= 2);
 }
 procedure headerAdd#send_length#3()
-  modifies C, R, M, I, H;
+  modifies C, R, M, I, H, I#sub;
 {
   var pl_bits: Chan (bv8);
   var data: Chan (bv8);
@@ -177,30 +190,32 @@ procedure headerAdd#send_length#3()
   var St: int;
   var pl_bits#0: bv8;
   assume (pl_bits != data) && (pl_bits != len) && (data != len);
-  assume 0 <= R[pl_bits];
-  assume 0 <= C[data];
-  assume 0 <= C[len];
+  assume HEADER_LEN == 5;
+  assume (0 <= I[pl_bits]) && (I[pl_bits] <= R[pl_bits]) && (R[pl_bits] <= C[pl_bits]);
+  assume (0 <= I[data]) && (I[data] <= R[data]) && (R[data] <= C[data]);
+  assume (0 <= I[len]) && (I[len] <= R[len]) && (R[len] <= C[len]);
   assume AT#BvUle8(0bv8, octet_index);
   assume AT#BvUle8(octet_index, octet_count);
   assume octet_count == 14bv8;
   assume (St == 1) ==> AT#BvUle8(octet_index, 5bv8);
   assume (St == 2) ==> AT#BvUlt8(5bv8, octet_index);
   assume (0 <= St) && (St <= 2);
-  assume !(true && AT#BvUlt8(octet_index, 5bv8) && (St == 1));
+  assume true;
+  assume !(AT#BvUlt8(octet_index, 5bv8) && (St == 1));
   assume (octet_index == 5bv8) && (St == 1);
   octet_index := AT#BvAdd8(octet_index, 1bv8);
   St := 2;
   M[data][C[data]] := AT#BvSub8(AT#BvSub8(octet_count, 5bv8), 1bv8);
   C[data] := C[data] + 1;
-  assert {:msg "25.12: Action at 69.2 might not preserve invariant (#18)"} AT#BvUle8(0bv8, octet_index);
-  assert {:msg "26.12: Action at 69.2 might not preserve invariant (#19)"} AT#BvUle8(octet_index, octet_count);
-  assert {:msg "27.12: Action at 69.2 might not preserve invariant (#20)"} octet_count == 14bv8;
-  assert {:msg "29.12: Action at 69.2 might not preserve invariant (#21)"} (St == 1) ==> AT#BvUle8(octet_index, 5bv8);
-  assert {:msg "30.12: Action at 69.2 might not preserve invariant (#22)"} (St == 2) ==> AT#BvUlt8(5bv8, octet_index);
-  assert {:msg "31.12: Action at 69.2 might not preserve invariant (#23)"} (0 <= St) && (St <= 2);
+  assert {:msg "headerAdd.cal(25.12): Action 'send_length' at headerAdd.cal(69.2) might not preserve the invariant (#18)"} AT#BvUle8(0bv8, octet_index);
+  assert {:msg "headerAdd.cal(26.12): Action 'send_length' at headerAdd.cal(69.2) might not preserve the invariant (#19)"} AT#BvUle8(octet_index, octet_count);
+  assert {:msg "headerAdd.cal(27.12): Action 'send_length' at headerAdd.cal(69.2) might not preserve the invariant (#20)"} octet_count == 14bv8;
+  assert {:msg "headerAdd.cal(29.12): Action 'send_length' at headerAdd.cal(69.2) might not preserve the invariant (#21)"} (St == 1) ==> AT#BvUle8(octet_index, 5bv8);
+  assert {:msg "headerAdd.cal(30.12): Action 'send_length' at headerAdd.cal(69.2) might not preserve the invariant (#22)"} (St == 2) ==> AT#BvUlt8(5bv8, octet_index);
+  assert {:msg "headerAdd.cal(31.12): Action 'send_length' at headerAdd.cal(69.2) might not preserve the invariant (#23)"} (0 <= St) && (St <= 2);
 }
 procedure headerAdd#send_payload_octet#4()
-  modifies C, R, M, I, H;
+  modifies C, R, M, I, H, I#sub;
 {
   var pl_bits: Chan (bv8);
   var data: Chan (bv8);
@@ -213,15 +228,17 @@ procedure headerAdd#send_payload_octet#4()
   var St: int;
   var pl_bits#0: bv8;
   assume (pl_bits != data) && (pl_bits != len) && (data != len);
-  assume 0 <= R[pl_bits];
-  assume 0 <= C[data];
-  assume 0 <= C[len];
+  assume HEADER_LEN == 5;
+  assume (0 <= I[pl_bits]) && (I[pl_bits] <= R[pl_bits]) && (R[pl_bits] <= C[pl_bits]);
+  assume (0 <= I[data]) && (I[data] <= R[data]) && (R[data] <= C[data]);
+  assume (0 <= I[len]) && (I[len] <= R[len]) && (R[len] <= C[len]);
   assume AT#BvUle8(0bv8, octet_index);
   assume AT#BvUle8(octet_index, octet_count);
   assume octet_count == 14bv8;
   assume (St == 1) ==> AT#BvUle8(octet_index, 5bv8);
   assume (St == 2) ==> AT#BvUlt8(5bv8, octet_index);
   assume (0 <= St) && (St <= 2);
+  assume 1 <= (C[pl_bits] - R[pl_bits]);
   pl_bits#0 := M[pl_bits][R[pl_bits]];
   R[pl_bits] := R[pl_bits] + 1;
   assume AT#BvUlt8(octet_index, octet_count) && (St == 2);
@@ -229,15 +246,15 @@ procedure headerAdd#send_payload_octet#4()
   St := 2;
   M[data][C[data]] := pl_bits#0;
   C[data] := C[data] + 1;
-  assert {:msg "25.12: Action at 80.2 might not preserve invariant (#24)"} AT#BvUle8(0bv8, octet_index);
-  assert {:msg "26.12: Action at 80.2 might not preserve invariant (#25)"} AT#BvUle8(octet_index, octet_count);
-  assert {:msg "27.12: Action at 80.2 might not preserve invariant (#26)"} octet_count == 14bv8;
-  assert {:msg "29.12: Action at 80.2 might not preserve invariant (#27)"} (St == 1) ==> AT#BvUle8(octet_index, 5bv8);
-  assert {:msg "30.12: Action at 80.2 might not preserve invariant (#28)"} (St == 2) ==> AT#BvUlt8(5bv8, octet_index);
-  assert {:msg "31.12: Action at 80.2 might not preserve invariant (#29)"} (0 <= St) && (St <= 2);
+  assert {:msg "headerAdd.cal(25.12): Action 'send_payload_octet' at headerAdd.cal(80.2) might not preserve the invariant (#24)"} AT#BvUle8(0bv8, octet_index);
+  assert {:msg "headerAdd.cal(26.12): Action 'send_payload_octet' at headerAdd.cal(80.2) might not preserve the invariant (#25)"} AT#BvUle8(octet_index, octet_count);
+  assert {:msg "headerAdd.cal(27.12): Action 'send_payload_octet' at headerAdd.cal(80.2) might not preserve the invariant (#26)"} octet_count == 14bv8;
+  assert {:msg "headerAdd.cal(29.12): Action 'send_payload_octet' at headerAdd.cal(80.2) might not preserve the invariant (#27)"} (St == 1) ==> AT#BvUle8(octet_index, 5bv8);
+  assert {:msg "headerAdd.cal(30.12): Action 'send_payload_octet' at headerAdd.cal(80.2) might not preserve the invariant (#28)"} (St == 2) ==> AT#BvUlt8(5bv8, octet_index);
+  assert {:msg "headerAdd.cal(31.12): Action 'send_payload_octet' at headerAdd.cal(80.2) might not preserve the invariant (#29)"} (0 <= St) && (St <= 2);
 }
 procedure headerAdd#done#5()
-  modifies C, R, M, I, H;
+  modifies C, R, M, I, H, I#sub;
 {
   var pl_bits: Chan (bv8);
   var data: Chan (bv8);
@@ -250,27 +267,29 @@ procedure headerAdd#done#5()
   var St: int;
   var pl_bits#0: bv8;
   assume (pl_bits != data) && (pl_bits != len) && (data != len);
-  assume 0 <= R[pl_bits];
-  assume 0 <= C[data];
-  assume 0 <= C[len];
+  assume HEADER_LEN == 5;
+  assume (0 <= I[pl_bits]) && (I[pl_bits] <= R[pl_bits]) && (R[pl_bits] <= C[pl_bits]);
+  assume (0 <= I[data]) && (I[data] <= R[data]) && (R[data] <= C[data]);
+  assume (0 <= I[len]) && (I[len] <= R[len]) && (R[len] <= C[len]);
   assume AT#BvUle8(0bv8, octet_index);
   assume AT#BvUle8(octet_index, octet_count);
   assume octet_count == 14bv8;
   assume (St == 1) ==> AT#BvUle8(octet_index, 5bv8);
   assume (St == 2) ==> AT#BvUlt8(5bv8, octet_index);
   assume (0 <= St) && (St <= 2);
-  assume !((1 <= (C[pl_bits] - R[pl_bits])) && AT#BvUlt8(octet_index, octet_count) && (St == 2));
+  assume true;
+  assume !(AT#BvUlt8(octet_index, octet_count) && (St == 2));
   assume (octet_index == octet_count) && (St == 2);
   St := 0;
-  assert {:msg "25.12: Action at 91.2 might not preserve invariant (#30)"} AT#BvUle8(0bv8, octet_index);
-  assert {:msg "26.12: Action at 91.2 might not preserve invariant (#31)"} AT#BvUle8(octet_index, octet_count);
-  assert {:msg "27.12: Action at 91.2 might not preserve invariant (#32)"} octet_count == 14bv8;
-  assert {:msg "29.12: Action at 91.2 might not preserve invariant (#33)"} (St == 1) ==> AT#BvUle8(octet_index, 5bv8);
-  assert {:msg "30.12: Action at 91.2 might not preserve invariant (#34)"} (St == 2) ==> AT#BvUlt8(5bv8, octet_index);
-  assert {:msg "31.12: Action at 91.2 might not preserve invariant (#35)"} (0 <= St) && (St <= 2);
+  assert {:msg "headerAdd.cal(25.12): Action 'done' at headerAdd.cal(91.2) might not preserve the invariant (#30)"} AT#BvUle8(0bv8, octet_index);
+  assert {:msg "headerAdd.cal(26.12): Action 'done' at headerAdd.cal(91.2) might not preserve the invariant (#31)"} AT#BvUle8(octet_index, octet_count);
+  assert {:msg "headerAdd.cal(27.12): Action 'done' at headerAdd.cal(91.2) might not preserve the invariant (#32)"} octet_count == 14bv8;
+  assert {:msg "headerAdd.cal(29.12): Action 'done' at headerAdd.cal(91.2) might not preserve the invariant (#33)"} (St == 1) ==> AT#BvUle8(octet_index, 5bv8);
+  assert {:msg "headerAdd.cal(30.12): Action 'done' at headerAdd.cal(91.2) might not preserve the invariant (#34)"} (St == 2) ==> AT#BvUlt8(5bv8, octet_index);
+  assert {:msg "headerAdd.cal(31.12): Action 'done' at headerAdd.cal(91.2) might not preserve the invariant (#35)"} (0 <= St) && (St <= 2);
 }
 procedure headerAdd##GuardWD#6()
-  modifies C, R, M, I, H;
+  modifies C, R, M, I, H, I#sub;
 {
   var pl_bits: Chan (bv8);
   var data: Chan (bv8);
@@ -283,14 +302,20 @@ procedure headerAdd##GuardWD#6()
   var St: int;
   var pl_bits#0: bv8;
   assume (pl_bits != data) && (pl_bits != len) && (data != len);
-  assert {:msg "1.1: The actions 'done' and 'get_data_len' of actor 'headerAdd' might not have mutually exclusive guards (#36)"} !(true && (!((1 <= (C[pl_bits] - R[pl_bits])) && AT#BvUlt8(octet_index, octet_count) && (St == 2))) && true && (octet_index == octet_count) && (St == 2) && true && (1 <= (C[pl_bits] - R[pl_bits])) && (St == 0));
-  assert {:msg "1.1: The actions 'done' and 'send_length' of actor 'headerAdd' might not have mutually exclusive guards (#37)"} !(true && (!((1 <= (C[pl_bits] - R[pl_bits])) && AT#BvUlt8(octet_index, octet_count) && (St == 2))) && true && (octet_index == octet_count) && (St == 2) && true && (!(true && AT#BvUlt8(octet_index, 5bv8) && (St == 1))) && true && (octet_index == 5bv8) && (St == 1));
-  assert {:msg "1.1: The actions 'done' and 'send_header' of actor 'headerAdd' might not have mutually exclusive guards (#38)"} !(true && (!((1 <= (C[pl_bits] - R[pl_bits])) && AT#BvUlt8(octet_index, octet_count) && (St == 2))) && true && (octet_index == octet_count) && (St == 2) && true && true && AT#BvUlt8(octet_index, 5bv8) && (St == 1));
-  assert {:msg "1.1: The actions 'done' and 'send_payload_octet' of actor 'headerAdd' might not have mutually exclusive guards (#39)"} !(true && (!((1 <= (C[pl_bits] - R[pl_bits])) && AT#BvUlt8(octet_index, octet_count) && (St == 2))) && true && (octet_index == octet_count) && (St == 2) && true && (1 <= (C[pl_bits] - R[pl_bits])) && AT#BvUlt8(octet_index, octet_count) && (St == 2));
-  assert {:msg "1.1: The actions 'get_data_len' and 'send_length' of actor 'headerAdd' might not have mutually exclusive guards (#40)"} !(true && (1 <= (C[pl_bits] - R[pl_bits])) && (St == 0) && true && (!(true && AT#BvUlt8(octet_index, 5bv8) && (St == 1))) && true && (octet_index == 5bv8) && (St == 1));
-  assert {:msg "1.1: The actions 'get_data_len' and 'send_header' of actor 'headerAdd' might not have mutually exclusive guards (#41)"} !(true && (1 <= (C[pl_bits] - R[pl_bits])) && (St == 0) && true && true && AT#BvUlt8(octet_index, 5bv8) && (St == 1));
-  assert {:msg "1.1: The actions 'get_data_len' and 'send_payload_octet' of actor 'headerAdd' might not have mutually exclusive guards (#42)"} !(true && (1 <= (C[pl_bits] - R[pl_bits])) && (St == 0) && true && (1 <= (C[pl_bits] - R[pl_bits])) && AT#BvUlt8(octet_index, octet_count) && (St == 2));
-  assert {:msg "1.1: The actions 'send_length' and 'send_header' of actor 'headerAdd' might not have mutually exclusive guards (#43)"} !(true && (!(true && AT#BvUlt8(octet_index, 5bv8) && (St == 1))) && true && (octet_index == 5bv8) && (St == 1) && true && true && AT#BvUlt8(octet_index, 5bv8) && (St == 1));
-  assert {:msg "1.1: The actions 'send_length' and 'send_payload_octet' of actor 'headerAdd' might not have mutually exclusive guards (#44)"} !(true && (!(true && AT#BvUlt8(octet_index, 5bv8) && (St == 1))) && true && (octet_index == 5bv8) && (St == 1) && true && (1 <= (C[pl_bits] - R[pl_bits])) && AT#BvUlt8(octet_index, octet_count) && (St == 2));
-  assert {:msg "1.1: The actions 'send_header' and 'send_payload_octet' of actor 'headerAdd' might not have mutually exclusive guards (#45)"} !(true && true && AT#BvUlt8(octet_index, 5bv8) && (St == 1) && true && (1 <= (C[pl_bits] - R[pl_bits])) && AT#BvUlt8(octet_index, octet_count) && (St == 2));
+  assume AT#BvUle8(0bv8, octet_index);
+  assume AT#BvUle8(octet_index, octet_count);
+  assume octet_count == 14bv8;
+  assume (St == 1) ==> AT#BvUle8(octet_index, 5bv8);
+  assume (St == 2) ==> AT#BvUlt8(5bv8, octet_index);
+  assume (0 <= St) && (St <= 2);
+  assert {:msg "headerAdd.cal(1.1): The actions 'send_header' and 'send_payload_octet' of actor 'headerAdd' might not have mutually exclusive guards (#36)"} !(true && true && AT#BvUlt8(octet_index, 5bv8) && (St == 1) && true && (1 <= (C[pl_bits] - R[pl_bits])) && AT#BvUlt8(octet_index, octet_count) && (St == 2));
+  assert {:msg "headerAdd.cal(1.1): The actions 'send_header' and 'get_data_len' of actor 'headerAdd' might not have mutually exclusive guards (#37)"} !(true && true && AT#BvUlt8(octet_index, 5bv8) && (St == 1) && true && (1 <= (C[pl_bits] - R[pl_bits])) && (St == 0));
+  assert {:msg "headerAdd.cal(1.1): The actions 'send_header' and 'done' of actor 'headerAdd' might not have mutually exclusive guards (#38)"} !(true && true && AT#BvUlt8(octet_index, 5bv8) && (St == 1) && true && (!((1 <= (C[pl_bits] - R[pl_bits])) && AT#BvUlt8(octet_index, octet_count) && (St == 2))) && true && (octet_index == octet_count) && (St == 2));
+  assert {:msg "headerAdd.cal(1.1): The actions 'send_header' and 'send_length' of actor 'headerAdd' might not have mutually exclusive guards (#39)"} !(true && true && AT#BvUlt8(octet_index, 5bv8) && (St == 1) && true && (!(true && AT#BvUlt8(octet_index, 5bv8) && (St == 1))) && true && (octet_index == 5bv8) && (St == 1));
+  assert {:msg "headerAdd.cal(1.1): The actions 'send_payload_octet' and 'get_data_len' of actor 'headerAdd' might not have mutually exclusive guards (#40)"} !(true && (1 <= (C[pl_bits] - R[pl_bits])) && AT#BvUlt8(octet_index, octet_count) && (St == 2) && true && (1 <= (C[pl_bits] - R[pl_bits])) && (St == 0));
+  assert {:msg "headerAdd.cal(1.1): The actions 'send_payload_octet' and 'done' of actor 'headerAdd' might not have mutually exclusive guards (#41)"} !(true && (1 <= (C[pl_bits] - R[pl_bits])) && AT#BvUlt8(octet_index, octet_count) && (St == 2) && true && (!((1 <= (C[pl_bits] - R[pl_bits])) && AT#BvUlt8(octet_index, octet_count) && (St == 2))) && true && (octet_index == octet_count) && (St == 2));
+  assert {:msg "headerAdd.cal(1.1): The actions 'send_payload_octet' and 'send_length' of actor 'headerAdd' might not have mutually exclusive guards (#42)"} !(true && (1 <= (C[pl_bits] - R[pl_bits])) && AT#BvUlt8(octet_index, octet_count) && (St == 2) && true && (!(true && AT#BvUlt8(octet_index, 5bv8) && (St == 1))) && true && (octet_index == 5bv8) && (St == 1));
+  assert {:msg "headerAdd.cal(1.1): The actions 'get_data_len' and 'done' of actor 'headerAdd' might not have mutually exclusive guards (#43)"} !(true && (1 <= (C[pl_bits] - R[pl_bits])) && (St == 0) && true && (!((1 <= (C[pl_bits] - R[pl_bits])) && AT#BvUlt8(octet_index, octet_count) && (St == 2))) && true && (octet_index == octet_count) && (St == 2));
+  assert {:msg "headerAdd.cal(1.1): The actions 'get_data_len' and 'send_length' of actor 'headerAdd' might not have mutually exclusive guards (#44)"} !(true && (1 <= (C[pl_bits] - R[pl_bits])) && (St == 0) && true && (!(true && AT#BvUlt8(octet_index, 5bv8) && (St == 1))) && true && (octet_index == 5bv8) && (St == 1));
+  assert {:msg "headerAdd.cal(1.1): The actions 'done' and 'send_length' of actor 'headerAdd' might not have mutually exclusive guards (#45)"} !(true && (!((1 <= (C[pl_bits] - R[pl_bits])) && AT#BvUlt8(octet_index, octet_count) && (St == 2))) && true && (octet_index == octet_count) && (St == 2) && true && (!(true && AT#BvUlt8(octet_index, 5bv8) && (St == 1))) && true && (octet_index == 5bv8) && (St == 1));
 }
